arm-hyp: remove unused ParityEnabled in aspec; solve sorries in ADT_H
ParityEnabled isn't used in ARM_HYP and we had to prove its absence as
invariant, which in turn makes the abstraction function from Haskell
to abstract partial (only works when invariants hold).

This commit removes that problem by removing ParityEnabled from the
abstract spec. Updated ainv and refine as necessary.

spec/abstract/ARM_HYP/Arch_Structs_A.thy
@@ -33,7 +33,7 @@ section {* Architecture-specific virtual memory *}
 text {* An ASID is simply a word. *}
 type_synonym asid = "word32"
 
-datatype vm_attribute = ParityEnabled | PageCacheable | XNever
+datatype vm_attribute = PageCacheable | XNever
 type_synonym vm_attributes = "vm_attribute set"
 
 section {* Architecture-specific capabilities *}
@@ -142,7 +142,7 @@ record  GICVCPUInterface =
   vgicHCR  :: machine_word
   vgicVMCR :: machine_word
   vgicAPR  :: machine_word
-  vgicLR   :: "nat \<rightharpoonup> ARM_A.virq"
+  vgicLR   :: "nat \<Rightarrow> ARM_A.virq"
 
 
 record vcpu =
@@ -172,7 +172,7 @@ where
       vgicHCR  = vgicHCREN,
       vgicVMCR = 0,
       vgicAPR  = 0,
-      vgicLR   = Map.empty \<rparr>" (* FIXME vgicLR *)
+      vgicLR   = \<lambda>_. 0 \<rparr>"
 
 definition
   default_vcpu :: vcpu where
