spec/abstract/ARM_HYP/VCPU_A.thy
@@ -184,7 +184,7 @@ where
      vcpu \<leftarrow> liftE $ get_vcpu p;
      vcpuLR \<leftarrow> returnOk (vgicLR $ vcpu_VGIC $ vcpu);
 
-     whenE (the (vcpuLR (unat index)) && vgic_irq_mask = vgic_irq_active) $ throwError DeleteFirst;
+     whenE (vcpuLR (unat index) && vgic_irq_mask = vgic_irq_active) $ throwError DeleteFirst;
 
      virq \<leftarrow> returnOk (make_virq group priority vid);
      returnOk $ InvokeVCPU $ VCPUInjectIRQ p (unat index) virq
@@ -198,7 +198,7 @@ where "invoke_vcpu_inject_irq vr index virq \<equiv> do
       Some (vr, _) \<Rightarrow> do_machine_op $ set_gic_vcpu_ctrl_lr (of_nat index) virq
     | None \<Rightarrow> do
            vcpu \<leftarrow> get_vcpu vr;
-           vcpuLR \<leftarrow> return (fun_upd (vgicLR $ vcpu_VGIC $ vcpu) index (Some virq));
+           vcpuLR \<leftarrow> return $ (vgicLR $ vcpu_VGIC vcpu) (index := virq);
            set_vcpu vr $ vcpu \<lparr> vcpu_VGIC := (vcpu_VGIC vcpu) \<lparr> vgicLR := vcpuLR \<rparr>\<rparr>
            od)
    od"
